tmap

dev.v
@@ -1,10 +1,24 @@
-From mathcomp Require Import ssreflect  ssrnat eqtype ssrbool ssrfun seq.
+From mathcomp Require Import ssreflect ssrnat eqtype ssrbool ssrfun seq.
+From mathcomp Require Import finmap choice finfun fintype.
+From deriving Require Import deriving.
 From coqspec Require Import int.
 
 Set Implicit Arguments.
 Unset Printing Implicit Defensive.
 
 Inductive Restr := Neq of Exp & Exp.
+
+Definition restr_indDef := [indDef for Restr_rect].
+Canonical restr_indType := IndType Restr restr_indDef.
+
+Definition restr_eqMixin := [derive eqMixin for Restr].
+Canonical restr_eqType := Eval hnf in EqType Restr restr_eqMixin.
+
+Definition br_indDef := [indDef for Branch_rect].
+Canonical br_indType := IndType Branch br_indDef.
+
+Definition br_eqMixin := [derive eqMixin for Branch].
+Canonical br_eqType := Eval hnf in EqType Branch br_eqMixin.
 
 Notation "e1 '≠' e2" := (Neq e1 e2) (at level 10).
 
@@ -18,25 +32,42 @@ Definition contr (r : Restr) :=
   | _                           => false
   end.
 
+Definition delete_restr (v : Var) := 
+  filter (fun '(r ≠ r') => (r != v) && (r' != v)).
 
-Definition contradict (c : Cenv) : bool :=
-  has contr c.2.
 
-Definition extend (c : Cenv) (b : Env) := 
-  let: (e, r) := c in (b ++ e, r).
+Definition contradict r : bool :=
+  has contr r.
+
+(*Definition extend (c : Cenv) (b : Env) := 
+  let: (e, r) := c in (e + b, r).*)
+
 
 Definition rsubst (r : seq Restr) (e : Env) : seq Restr := 
   map (fun '(r1 ≠ r2) => r1 /s/ e ≠ r2 /s/ e) r.
 
+Inductive Bind := BIND of Var & Exp.
+Notation "v ↦ e" := (BIND v e) (at level 20).
+
+Definition extend (c : Cenv) (b : Bind) : Cenv := 
+  let: (ce, rs) := c in
+  let: (v ↦ e)  := b in
+  ([fsfun ce with v |-> e], rs).
+
+Definition of_Bind : Bind -> Env := 
+  fun '(k ↦ e) => [fsfun emsub with k |-> e].
+
+Coercion of_Bind : Bind >-> Env.
+
 Definition b2r : Bind -> Restr := fun '(a ↦ b) => a ≠ b.
+Coercion b2r : Bind >-> Restr.
 
 Definition csubst (c : Cenv) (e : Env) := 
   let: (ce, r) := c in
-  (map (fun '(v ↦ x) => v ↦ (subst x e)) ce, rsubst r e).
+  (comp e ce, rsubst r e).
 
 Definition restr (c : Cenv) (b : Bind) := 
-  let: (e, r) := c in
-  (e, b2r b :: r).
+  let: (e, r) := c in (e, b2r b :: r).
 
 Inductive CBranch := 
   | CTRUE  of Cenv
@@ -44,9 +75,9 @@ Inductive CBranch :=
   | CBOTH  of Cntr & Cenv & Cenv.
 
 Definition both (c : Cntr) (te fe : Cenv) (b : Bind) :=
-  let: e1 := csubst te [:: b] in
+  let: e1 := csubst te b in
   let: e2 := restr  fe b in
-  if contradict e1 then
+  if contradict e1.2 then
     CFALSE e2
   else CBOTH c e1 e2.
 
@@ -56,27 +87,39 @@ Definition dev_cntr (c : Cntr) (ce : Cenv) : CBranch :=
     let: x' := x /s/ (ce.1) in
     let: y' := y /s/ (ce.1) in
     match x', y' with
-    | Arg_Val 'a, Arg_Val 'b
-    | Arg_Var a,  Arg_Var b  => if a == b then CTRUE ce else CFALSE ce
-    | Arg_Var v, Arg_Val u   => 
+    | Arg_Val 'a, Arg_Val 'b => if a == b then CTRUE ce else CFALSE ce
+    | Arg_Var a,  Arg_Var b  => 
+      if a == b then 
+        CTRUE ce 
+      else both (EQA? (Arg_Var a) (Arg_Var b)) ce ce (a ↦ b)
+    | Arg_Var v,  Arg_Val u  => 
       both (EQA? (Arg_Var v) (Arg_Val u)) ce ce (v ↦ y')
-    | Arg_Val u, Arg_Var v   => 
-      both (EQA? (Arg_Val u) (Arg_Var v)) ce ce (v ↦ y')
-    | _, _ => CFALSE ce 
+    | Arg_Val u,  Arg_Var v  => 
+      both (EQA? (Arg_Val u) (Arg_Var v)) ce ce (v ↦ x')
+    | _, _                   => CBOTH (EQA? x' y') ce ce
     end
-  | CONS? x h t =>
-    let: x' := x /s/ (ce.1) in
+  | CONS? x h t pf =>
+    let: e := extend (extend ce (t ↦ '0)) (h ↦ '0) in
+    let: x' := x /s/ (e.1) in
     match x' with
-    | CONS a b  => CTRUE (extend ce ((h ↦ a) :: [:: t ↦ b]))
-    | Arg_Val _ => CFALSE ce
-    | Arg_Var v => both (CONS? v h t) ce ce (v ↦ CONS h t)
+    | CONS a b  => CTRUE 
+      (extend (extend e (t ↦ b)) (h ↦ a))
+    | Arg_Val _ => CFALSE e
+    | Arg_Var v => 
+       let (e0, rs) := e in
+       both (CONS? v h t pf)
+        ([fsfun e0 with h |->  Exp_Arg h, t |-> Exp_Arg t],
+        delete_restr t (delete_restr h rs))
+        ce
+        (v ↦ CONS h t)
     end
   end.
 
 Fixpoint dev (t : Tree) (e : Cenv) : Tree :=
   match t with
   | RET x        => x /s/ (e.1)
-  | LET v x t    => dev t (extend e [:: v ↦ x /s/ (e.1)])
+  | LET v x t    => 
+    dev t (extend e (v ↦ x /s/ ([fsfun e.1 with v |-> Exp_Arg '0])))
   | COND c t1 t2 => 
     match dev_cntr c e with
     | CTRUE e       => dev t1 e
@@ -88,10 +131,473 @@ Fixpoint dev (t : Tree) (e : Cenv) : Tree :=
 Definition dev_Prog (f : Prog) (e : seq Exp) := 
   let: DEFINE n vs t := f in
   let: s := size e in
-  DEFINE n (drop s vs) (dev t (zip vs e, [::])).
+  DEFINE n (drop s vs) (dev t (fmap_of vs e, [::])).
 
-Theorem int_dev (p : Prog) (e1 e2 : seq Exp): 
-  let: DEFINE n vs t := p in
-  size e1 + size e2 = size vs ->
-  int_Prog p (e1 ++ e2) = int_Prog (dev_Prog p e1) e2.
+Section SubstTh.
+
+Lemma substE (e1 e2 : Env) : 
+  (forall v : Var, v /s/ e1 = v /s/ e2) -> e1 = e2.
+Proof.
+by move=> E; apply/fsfunP=> [[n]]; move: (E (VAR n)).
+Qed.
+
+Lemma substP (f : Exp -> Exp) (env : Env): 
+  (forall v : Var, env v = f v) ->
+  (forall a, f 'a = 'a) ->
+  (forall e1 e2, f (CONS e1 e2) = CONS (f e1) (f e2)) ->
+  (forall e, e /s/ env = f e).
+Proof.
+move=> ???; elim=> /= [[[]|?]|?->?->]//=.
+Qed.
+
+
+Lemma fsfunE {K : choiceType} {V : eqType} S f y dflt: 
+  ([fsfun x in S => f x] : {fsfun K -> V for dflt}) y = 
+  if y \in S then f y else dflt y.
+Proof. 
+rewrite /fsfun_of_fun /fsfun_of_ffun Fsfun.of_ffunE.
+by case: insubP=> [[/=??->->]|/negbTE->].
+Qed.
+
+Lemma emsubv v: 
+  emsub v = v.
+Proof. by rewrite fsfun_dflt /= ?finsupp0 ?inE. Qed.
+
+
+Lemma comp_env x e1 e2: 
+  x /s/ (comp e1 e2) = (x /s/ e1) /s/ e2.
+Proof.
+rewrite -[(x /s/ e1) /s/ e2]/((fun y => (y /s/ e1) /s/ e2) x).
+apply/substP=> // ?.
+rewrite /comp fsfunE; case: ifP=> //= /negbT.
+by rewrite inE negb_or => /andP[??]; rewrite fsfun_dflt //= fsfun_dflt.
+Qed.
+
+Lemma comp_var e1 e2 v : comp e1 e2 v = (e1 v) /s/ e2.
 Proof. Admitted.
+
+
+Lemma comp0e e1: comp emsub e1 = e1.
+Proof. by apply/substE=> v; rewrite comp_env /= emsubv. Qed.
+
+Lemma compe0 e1: comp e1 emsub = e1.
+Proof. 
+apply/substE=> v. rewrite comp_env /= -{2}[e1 v]/(id (e1 v)).
+apply/substP=> //; exact/emsubv.
+Qed.
+
+Lemma compA e1 e2 e3 : comp e1 (comp e2 e3) = comp (comp e1 e2) e3.
+Proof. by apply/substE=> ?; rewrite ?comp_env. Qed.
+  
+Lemma subst_var (v u : Var) (e : Exp): 
+  v /s/ ([fsfun emsub with u |-> e]) = if v == u then e else v.
+Proof. by rewrite /= fsfun_withE emsubv. Qed.
+
+Lemma rsubst2 rs e1 e2: 
+ rsubst (rsubst rs e1) e2 = rsubst rs (comp e1 e2).
+Proof.
+rewrite /rsubst -map_comp/=; apply eq_map=> [[]]/=*; by rewrite -?comp_env.
+Qed. 
+
+Lemma contradict_rsubstP e1 rs: 
+  reflect 
+  (exists r1 r2, ((r1 ≠ r2) \in rs) * (contr (r1 /s/ e1 ≠ r2 /s/ e1)))%type
+  (contradict (rsubst rs e1)).
+Proof.
+apply/(equivP hasP); split=> [[[?? /mapP[[r1 r2 ? -> ?]]]]|[r1 [r2 [*]]]].
+- by exists r1, r2.
+exists (r1 /s/ e1 ≠ r2 /s/ e1)=> //; by apply/mapP; exists (r1 ≠ r2).
+Qed.
+
+Lemma Ncontradict_rsubstP e1 rs: 
+  reflect 
+  (forall r1 r2, ((r1 ≠ r2) \in rs) -> (~~ contr (r1 /s/ e1 ≠ r2 /s/ e1)))%type
+  (~~ contradict (rsubst rs e1)).
+Proof.
+apply/(equivP hasPn); split=> [R r1 r2 ?|R [r1 r2 /mapP[[e e0 /R + ->]]]]//.
+by apply/R/mapP; exists (r1 ≠ r2).
+Qed.
+
+Lemma contradict_rsubst {e1 rs}: 
+  ~~ contradict (rsubst rs e1) ->
+  ~~ contradict rs.
+Proof.
+move/Ncontradict_rsubstP=> C; apply/hasPn=> [[++/C]].
+case=> [[[]?[[[]|]|]|u[[]|]]|??[]]// v.
+case: (boolP (u == v))=> [|/negbTE/=->]// /eqP->/=.
+case: (e1 v)=> // [[[]|]] ?; by rewrite eq_refl.
+Qed.
+
+Lemma subst_with e1 e2 e3:
+  closed_sub e2 -> 
+  finsupp e3 `<=` finsupp e2 ->
+  e1 /s/ e2 = (e1 /s/ e2) /s/ e3.
+Proof.
+move=> C /fsubsetP V.
+rewrite -[(e1 /s/ e2) /s/ e3]/((fun x => (x /s/ e2) /s/ e3) e1).
+apply/substP=> //= v.
+case: (boolP (v \in finsupp e2))=> [/C|/[dup] /negP N N'].
+- elim: (e2 v)=> [[[]|[]n /eqP/(congr1 (fun x => #|` x|))]|]//=.
+- by rewrite cardfs1.
+- move=> ? IHe1 ? IHe2. 
+  by rewrite /closed /= fsetU_eq0=> /andP[]/IHe1{1}->/IHe2{1}->.
+by rewrite fsfun_dflt //=  fsfun_dflt //; apply/negP=> /V /N.
+Qed.
+
+Lemma emsub_with (v : Var) : [fsfun emsub with v |-> Exp_Arg v] = emsub.
+Proof.
+by apply/substE=> /= ?; rewrite fsfun_withE emsubv; case: ifP=> [/eqP->|].
+Qed.
+
+Lemma sub_emsub e : e /s/ emsub = e.
+Proof. rewrite -[e]/(id e); apply/substP=> //; exact/emsubv. Qed.
+
+
+End SubstTh.
+
+Lemma contr_symm r1 r2: 
+  contr (r1 ≠ r2) = contr (r2 ≠ r1).
+Proof.
+case: r1 r2=> [[[]|]|??[[[]|]|]]//.
+- move=> ? []// [[]|] // ? /=; exact/esym.
+move=> ? []// [[]|]// ? /=; exact/esym.
+Qed.
+
+Lemma contrrr r: 
+  contr (r ≠ r).
+Proof. by case: r=> // [[[]|]] ? /=; rewrite eq_refl. Qed.
+
+Lemma NCTRUEboth c e1 e2 b e3 :
+  ~ both c e1 e2 b = CTRUE e3.
+Proof. by rewrite /both; case: ifP. Qed.
+
+Lemma contradict_ATOM {v : Var} {u : Arg} {e1 e2 rs e}: 
+  ~~ (contradict (rsubst rs e2)) ->
+  both (EQA? v u) (e1, rs) (e1, rs) (v ↦ u) = CFALSE e ->
+  (~~ contr (v /s/ e2 ≠ (u /s/ e2)) * (e = (e1, v ≠ u :: rs))).
+Proof.
+rewrite /both; case: ifP=> // [++[->]].
+case/contradict_rsubstP=> r1 [r2 [++ /Ncontradict_rsubstP I]].
+move: r1 r2=> ++ /I.
+case=> [[[]|]|??[[[]|?]|]]//; rewrite ?subst_var; last by case: ifP.
+- move=> a [] // [[]/=? /negbTE->|] // ?; rewrite subst_var; case: ifP=> //= /eqP->.
+  case: u=> // [[? + /eqP <-]] //=; case: (e2 v)=> // [[]] // [?]; by rewrite eq_sym.
+move=> ? [[[]|]|]//; last (rewrite subst_var; case: ifP=> // /eqP->).
+- case: u=> [|??]; last by (rewrite subst_var; case: ifP).
+  by move=> []??; rewrite subst_var; case: ifP=> // /eqP-> /[swap] /eqP->.
+  move=> ?; rewrite ?subst_var; case: ifP; case: ifP=> //.
+  - by move/eqP->=> /eqP->; rewrite contrrr.
+  - by move=> ? /eqP->; case: u=> [[]|]// ?? /eqP->.
+  - by move/eqP->; case: u=> [[]|]// ? ? + /eqP<-; rewrite contr_symm.
+  by move=> +++ /eqP E; rewrite E contrrr.
+by case: u=> // [[]]//.
+Qed.
+
+Lemma contradict_ATOM' {v : Var} {u : Arg} {e1 e2 rs e}: 
+  ~~ (contradict (rsubst rs e2)) ->
+  both (EQA? u v) (e1, rs) (e1, rs) (v ↦ u) = CFALSE e ->
+  (~~ contr (v /s/ e2 ≠ (u /s/ e2)) * (e = (e1, v ≠ u :: rs))).
+Proof.
+rewrite /both; case: ifP=> // [++[->]].
+case/contradict_rsubstP=> r1 [r2 [++ /Ncontradict_rsubstP I]].
+move: r1 r2=> ++ /I.
+case=> [[[]|]|??[[[]|?]|]]//; rewrite ?subst_var; last by case: ifP.
+- move=> a [] // [[]/=? /negbTE->|] // ?; rewrite subst_var; case: ifP=> //= /eqP->.
+  case: u=> // [[? + /eqP <-]] //=; case: (e2 v)=> // [[]] // [?]; by rewrite eq_sym.
+move=> ? [[[]|]|]//; last (rewrite subst_var; case: ifP=> // /eqP->).
+- case: u=> [|??]; last by (rewrite subst_var; case: ifP).
+  by move=> []??; rewrite subst_var; case: ifP=> // /eqP-> /[swap] /eqP->.
+  move=> ?; rewrite ?subst_var; case: ifP; case: ifP=> //.
+  - by move/eqP->=> /eqP->; rewrite contrrr.
+  - by move=> ? /eqP->; case: u=> [[]|]// ?? /eqP->.
+  - by move/eqP->; case: u=> [[]|]// ? ? + /eqP<-; rewrite contr_symm.
+  by move=> +++ /eqP E; rewrite E contrrr.
+by case: u=> // [[]]//.
+Qed.
+
+Lemma dev_contr_CTRUE e2 {e1 : Env}
+  {rs : seq Restr} {e : Cenv} {c : Cntr}:
+  (closed_sub e2) -> 
+  (closed_sub (comp e1 e2)) ->
+  cntr c (comp e1 e2) <> ERR ->
+  dev_cntr c (e1, rs) = CTRUE e ->
+  ((cntr c (comp e1 e2) = TRUE (comp e.1 e2)) *
+  (e.2 = rs))%type.
+Proof.
+move=> CL F.
+case: c => /= [[[]|????]|]//=.
+  rewrite ?fsfun_withE; case: ifP=> [/eqP->|].
+  - rewrite ?comp_var ?fsfun_with //=.
+  case: ifP=> [/eqP-> UV1|]; first rewrite comp_var fsfun_withE UV1 fsfun_with //.
+  move=> VU VV1; rewrite ?comp_var /= fsfun_withE VV1 fsfun_withE VU.
+- case E: (e1 _)=> //= [a|].
+  - case: a E=> [[]|?]//; rewrite /= ?fsfun_withE ?emsubv; case: ifP=> //; case: ifP=> //.
+    move=> ??? + /NCTRUEboth//.
+  - move=> ? [<-] /=; split=> //; apply/congr1.
+  - apply/substE=> ?; rewrite ?comp_env /= ?fsfun_withE.
+    case: ifP=> [/eqP<-|]. rewrite ?fsfun_with. admit.
+    (*rewrite -[(_ /s/ e2) /s/ _]subst_with // -subst_with //.*)
+  (*rewrite ?fsfun_withE emsubv=> ->; case: ifP=> //.*)
+  (*rewrite -[(_ /s/ e2) /s/ _]subst_with // -subst_with //.*)
+  admit.
+rewrite ?comp_env.
+case E: (_ /s/ e1)=> [[[]/=|]|]; rewrite ?comp_env //.
+case E': (_ /s/ e1)=> // [[[]|]]/=.
+- by case: ifP=> //= ?? [<-].
+- by move=> + /NCTRUEboth.
+case E': (_ /s/ e1)=> [[|]|] //.
+- by move=> +/NCTRUEboth.
+- case: ifP=> [/eqP-> + [<-]|? + /NCTRUEboth]//.
+case E1: (_ /s/ _)=> [[][]|]; by rewrite ?eq_refl.
+Admitted.
+
+Lemma memdel r v rs: 
+  r \in delete_restr v rs -> r \in rs.
+Proof. by rewrite /delete_restr mem_filter=> /andP[]. Qed.
+
+Lemma dev_contr_CFALSE e2 {e1 : Env}
+  {rs : seq Restr} {e : Cenv} {c : Cntr}:
+  cntr c (comp e1 e2) <> ERR ->
+  ~~ contradict (rsubst rs e2) ->
+  dev_cntr c (e1, rs) = CFALSE e ->
+  ((cntr c (comp e1 e2) = FALSE (comp e.1 e2)) *
+  ~~ contradict (rsubst e.2 e2))%type.
+Proof.
+case: c=> /= [??? ++ C|?? + C].
+- case E: (_ /s/ e1)=> [[[]|v]|]//; rewrite ?comp_env E /=.
+  - by move=> ? + [<-].
+  move=> ?.
+  rewrite /both; case: ifP=> //= /contradict_rsubstP[r1[r2[]]].
+  move/memdel/memdel=> /[dup] I.
+  move/Ncontradict_rsubstP: (C) => /[apply].
+  move/contradict_rsubst: (C); rewrite /contradict -all_predC=> /allP/(_ _ I).
+  case: ifP=> [?|].
+  case: r1 {I}=> [[[]|]|].
+  - case: r2=> [[[]/= ?? /negbTE->|]|]//.
+    move=> ??; rewrite subst_var; by case: ifP.
+  - case: r2=> [[[]??|v1 v2]|?? v1].
+    - rewrite subst_var; by case: ifP.
+    rewrite ?subst_var; case: ifP; case:ifP=> //.
+    - by move=> /eqP->/eqP->/eqP.
+    by move=> ?? /negbTE->.
+  - rewrite subst_var; case: ifP=> // /eqP->.
+  case S : (e2 v)=> [a|]//=; rewrite ?S //.
+  move=> _ _ ? + [<-]; split=> //=; rewrite ?S.
+  by case: a {S}=> [[]|]/=; rewrite ?S //.
+- case: r2=> [[[]|]|]// ???.
+  rewrite subst_var; case: ifP=> // /eqP->.
+  case S : (e2 v)=> [a|]//=; rewrite ?S //.
+  move=> _ _ ? + [<-]; split=> //=; rewrite S.
+  by case: a {S}=> [[]|]/=.
+- by rewrite emsub_with ?sub_emsub=> ? /negbTE->.
+rewrite ?comp_env; case: (_ /s/ e1)=> //.
+case=> [[]a|]/=.
+- case: (_ /s/ e1)=> [[[]?|]|//] //=.
+  - case: ifP=> // N + [<-]//.
+  move=> ? + /(contradict_ATOM' C) [+ ->]/=.
+  move=> /=; case: (e2 _)=> [[][]|]//=.
+  move=> ? + /negbTE N; by rewrite eq_sym N.
+move=> v; case: (_ /s/ e1)=> //.
+- case=> [[]? H /(contradict_ATOM C)/= [E ->]|?]; last case: ifP=> // ?.
+  - split=> /=; move: E H; case: (e2 _)=> //.
+    - move=> [[]|]// ?; by case: ifP=> // /eqP->/eqP.
+    case=> [][]// ?; rewrite negb_or C andbT=> +?; apply/implyP; rewrite implybNN.
+    by apply/implyP=> /eqP->.
+  move=> + /(contradict_ATOM C)/=[V->]; split=>/=.
+  - move: H; case E: (e2 v)=> // [[[]|]]//=.
+    - case E': (e2 _)=> // [[[]|]]//; case: ifP=> // /eqP A.
+      by rewrite E E' A /= eq_refl in V.
+  - move: H; case E': (e2 _)=> // [[[]|]]//=.
+    case E: (e2 _)=> // [[[]|]]//; case: ifP=> // /eqP N.
+    by rewrite E E' /= N eq_refl in V.
+Qed.
+
+Definition good (e : Env) := 
+  forall v u : Var, v \in finsupp e -> e v = u -> u \notin finsupp e.
+
+
+Lemma dev_contr_CBOTH1 {e2 e1 : Env}
+  {rs rs1 : seq Restr} {ce1 : Env} {ce2 : Cenv}
+  (c c1: Cntr) (e : Env): 
+  (closed_sub e2) ->
+  (good e1) ->
+  ~~ contradict (rsubst rs e2) ->
+  (cntr c (comp e1 e2)) <> ERR ->
+  dev_cntr c (e1, rs) = CBOTH c1 (ce1, rs1) ce2 ->
+  cntr c1 e2 = TRUE e ->
+  (
+    (cntr c (comp e1 e2) = TRUE (comp ce1 e)) *
+    (~~ contradict (rsubst rs1 e))
+  )%type.
+Proof.
+move=> CL C G; case: c=> /= [? v v1|??]; rewrite ?comp_env.
+- case E: (_ /s/ e1)=> // [[[]|]v2] // ; rewrite /both.
+  move=> /[dup] /negbTE; rewrite {1}eq_sym=> NV ?.
+  case: ifP=> //= ? + [<-<-<-] /=. case E' : (e2 _)=> //=[?].
+  move=> _ ? [<-]; split.
+  - apply/congr1/substE=> u; rewrite ?comp_env.
+    case: (boolP (u == v2))=> [/eqP->|/negbTE NE].
+    - case: ifP=> [/andP[/negbTE V2V /negbTE V2V1]|NE].
+      - rewrite /= fsfun_with /= fsfun_with /= fsfun_with.
+        rewrite ?fsfun_withE NV eq_refl /= ?fsfun_withE NV eq_refl ?emsubv.
+        rewrite V2V V2V1. admit. (* goodness *)
+      - rewrite /= fsfun_with /= ?fsfun_withE emsubv; case: ifP.
+        - rewrite /= fsfun_with. admit. (* e2 closed *)
+        move=> V2V; rewrite V2V /= in NE; move/negbT: NE; case: ifP=> //.
+        move/eqP<-; rewrite /= fsfun_withE V2V fsfun_with. admit. (* e2 closed *)
+      rewrite /= ?fsfun_withE NE emsubv /= ?fsfun_withE; move: (NV). 
+      case: ifP.
+      - rewrite /= fsfun_with. admit. (* closed e2 *)
+      case: ifP=> /=.
+      - rewrite fsfun_withE NV fsfun_with. (* closed e2 *) admit.
+      admit.
+      admit.
+case E: (_ /s/ e1)=> [[[]|]|]//=. 
+- case E': (_ /s/ e1)=> [[[]|]|] //; first by case: ifP.
+  - rewrite/both; case: ifP=> //= ? + [<-<-<-?/=].
+    case E1: (e2 _)=> //[[[]|]]//; case: ifP=> // ? + [<-]; split.
+    apply/congr1.
+    apply/substE=> ?; rewrite ?comp_env /= fsfun_withE emsubv; case: ifP=> //=.
+    move/eqP=>->. (* goodnes e1 *) admit. 
+    admit.
+- case E': (_ /s/ e1)=> /= [[[]|]|]//=.
+  - rewrite /both; case: ifP=> //= ? + [<-<-<-/= ?].
+    case E1: (e2 _)=> // [[[]|]]//; case: ifP=> //.
+    move/eqP=> A ? [<-]; split.
+    - apply/congr1/substE=> ?; rewrite ?comp_env /= fsfun_withE emsubv.
+      case: ifP=> /= [/eqP->|] //. (* goodnes e1 *) admit.
+    admit.
+  - case: ifP=> // + ?; rewrite /both; case: ifP=> // ? + [<-<-<-]/=.
+    case E1: (e2 _)=> /= [[[]|]|] //.
+    - case E2: (e2 _)=> // [[[]|]]//; case: ifP=> //.
+      move=> ??? [<-]. split.
+      - apply/congr1/substE=> ?; rewrite ?comp_env /= fsfun_withE emsubv.
+        case: ifP=> /= [/eqP->|] //. (* goodeness e1 *) admit.
+      admit.
+    case E2: (e2 _)=> // [[[]|]]//; case: ifP=> //.
+Admitted.
+
+Lemma dev_contr_CBOTH2 {e2 e1 : Env}
+  {rs rs1 : seq Restr} {ce1 : Env} {ce2 : Cenv}
+  {c c1: Cntr} {e : Env}: 
+  ~~ contradict (rsubst rs e2) ->
+  (cntr c (comp e1 e2)) <> ERR ->
+  dev_cntr c (e1, rs) = CBOTH c1 ce2 (ce1, rs1) ->
+  cntr c1 e2 = FALSE e ->
+  (
+    (cntr c (comp e1 e2) = FALSE (comp ce1 e)) *
+    (~~ contradict (rsubst rs1 e2))
+  )%type.
+Proof.
+move=> C; case: c=> /= [???|??]; rewrite ?comp_env.
+case E: (_ /s/ e1)=> [[[]|]|]//=.
+move=> ?. 
+- rewrite/both; case: ifP=> //= ? + [<-?<-<-]/=.
+  case: (e2 _)=> // [[[]??[<-]|??[<-]]]//.
+  case: ifP=> //=.
+- case: (_ /s/ e1)=> [[[]|]|]//=.
+  case: (_ /s/ e1)=> [[[]|]|]//= ??; first by case:ifP.
+  rewrite /both; case: ifP=> //= ? + [<-?<-<-]/=.
+  case: (e2 _)=> // [[]] // [] ?; case: ifP=> [/eqP-> ?|] //.
+  move=> N ? [<-]; by rewrite eq_sym N.
+- case: (_ /s/ e1)=> [[[]|]|???+[<-?<-<-]]/=.
+  - move=> ??; rewrite /both /=; case: ifP=> //= ? + [<-?<-<-/=].
+    case: (e2 _)=> // [[]] // [] ?; by case: ifP=> // ? + [<-].
+  move=> ??; case: ifP => // ? +; rewrite/both; case: ifP=> //.
+  move=> N + [<-?<-<-]/=; case: (e2 _)=> [[]// []|??] //.
+  by case: (e2 _)=> // [[]] // [] ??; case: ifP=> // ?? [<-].
+by case: (e2 _)=> [] // [] // [] /=.
+Qed.
+
+Lemma dev_contr_CBOTH3 {e2 e1 : Env}
+  {rs rs1 : seq Restr} {ce1 : Env} {ce2 : Cenv}
+  {c c1: Cntr}: 
+  (cntr c (comp e1 e2)) <> ERR ->
+  dev_cntr c (e1, rs) = CBOTH c1 ce2 (ce1, rs1) ->
+  cntr c1 e2 = ERR -> False.
+Proof.
+case: c=> [a??|??]/=; rewrite ?comp_env.
+- case: (_ /s/ e1)=> // [[]] // ???; rewrite /both.
+  by case: ifP=> // ? [<-?] /=; case: (e2 _).
+case: (_ /s/ e1)=> // [[[]|]]/=.
+- case: (_ /s/ e1)=> []// [[]|]/= ??; first by case: ifP.
+- rewrite /both; case: ifP => // ? + [<-?] /=.
+  case: (e2 _)=> // [[]] // [] ?; by case: ifP.
+case: (_ /s/ e1)=> [[[]|]|???+[<-]] /=.
+- move=> ??; rewrite /both; case: ifP=> // ? + [<-]/=.
+  case: (e2 _)=> // [[]] // [] ?; by case: ifP.
+- move=> ??; case: ifP=> // ?; rewrite /both; case: ifP=> // ? + [<-] /=.
+  case: (e2 _)=> // [[]] // [] ?; case: (e2 _)=> // [[]] // [] ?.
+  by case: ifP.
+by case: (e2 _).
+Qed.
+
+Lemma int_dev (t : Tree) (e1 e2 : Env) (rs : seq Restr): 
+  (closed_sub e2) ->
+  int t (comp e1 e2) <> '0 ->
+  ~~ contradict (rsubst rs e2) ->
+  int t (comp e1 e2) = int (dev t (e1, rs)) e2.
+Proof.
+elim: t e1 e2 rs=> //= [*|t e ?|c t1 IHt1 t2 IHt2 e1 e2 ? CL C CR].
+- by rewrite comp_env.
+- move => IHt /= e1 e2 ?? NE ?.
+  have H: [fsfun comp e1 e2 with t |-> e /s/ ([fsfun comp e1 e2 with t |-> Exp_Arg '0])] =
+  comp [fsfun e1 with t |-> e /s/ ([fsfun e1 with t |-> Exp_Arg '0])] e2.
+  - apply/substE=> u; rewrite comp_env /=.
+    rewrite ?fsfun_withE; case: ifP=> [?|?].
+    - suff ->: [fsfun comp e1 e2 with t |-> Exp_Arg ' (0)] =
+            comp [fsfun e1 with t |-> Exp_Arg ' (0)] e2.
+      - by rewrite comp_env.
+    apply/substE=> u'; rewrite comp_env /= ?fsfun_withE; case: ifP=> //.
+    - by rewrite -[comp e1 e2 u']/(u' /s/ (comp e1 e2)) comp_env.
+    by rewrite -[comp e1 e2 u]/(u /s/ (comp e1 e2)) comp_env.
+  by rewrite -IHt // -H.
+have NE : (cntr c (comp e1 e2) <> ERR) by move: C; case: (cntr _).
+case E : (dev_cntr _ _)=> [[]|[]|?[]??[]]/=.
+- move/(dev_contr_CTRUE CL NE): E C=>/=[->->] ?.
+  by rewrite -IHt1.
+- move/(dev_contr_CFALSE e2 NE CR): E C=>/= [-> ?] ?.
+  by rewrite -IHt2.
+case E': (cntr _ e2).
+- move: E' C=> /[dup] /(dev_contr_CBOTH1 _ CL CR NE E)[->].
+  move=> ? /cntr_env_TRUE/(_ CL)[] *; by rewrite -IHt1.
+- move: E' C=> /[dup] /(dev_contr_CBOTH2 CR NE E)[->].
+  move=> ? /cntr_env_FALSE /eqP -> ?; by rewrite -IHt2.
+by move/(dev_contr_CBOTH3 NE E): E'.
+Admitted.
+
+Lemma foldr_monoid {T : Type} {f : T -> T -> T} {n s1 s2}: 
+  associative f ->
+  (forall x, f n x = x) ->
+  (forall x, f x n = x) ->
+  f (foldr f n s1) (foldr f n s2) =
+  foldr f n (s1 ++ s2).
+Proof. by move=> A L R; elim: s1=> //= ??; rewrite -A=>->. Qed.
+
+
+Lemma fmap_cat e1 e2 t:
+  size t = (size e1 + size e2)%N  ->
+  fmap_of t (e1 ++ e2) =
+  comp (fmap_of t e1) (fmap_of (drop (size e1) t) e2).
+Proof.
+  move=> E.
+  rewrite /fmap_of (foldr_monoid compA comp0e compe0); apply/congr1.
+  rewrite -map_cat -{1}(cat_take_drop (size e1) t) zip_cat.
+  apply/congr1/congr2=> //.
+  - rewrite -{3}(cats0 e1) -{2}(cat_take_drop (size e1) t) zip_cat.
+    by case: (drop _)=> /=; rewrite cats0.
+all: by rewrite size_takel // E -{1}(addn0 (size e1)) leq_add2l leq0n. 
+Qed.
+
+Theorem int_dev_Prog (p : Prog) (e1 e2 : seq Exp):
+  let: DEFINE n vs t := p in
+  (size e1 + size e2)%N = size vs ->
+  (forall x, x \in e2 -> closed x) ->
+  int_Prog p (e1 ++ e2) <> '0 ->
+  int_Prog p (e1 ++ e2) = int_Prog (dev_Prog p e1) e2.
+Proof. 
+case: p=> /= _ ??? H ?.
+by rewrite -int_dev // -?fmap_cat // => ? /codomf_fmap_of/H.
+Qed.
+
+
